checkpoint

ml/Atom.ml
@@ -1,0 +1,110 @@
+;; open StringLib
+
+(*
+  This is a type for "finite sets" with some structure.  Atom.t forms a total order
+  and we can therefore put them into Set data structures.
+
+  Morally, we will think of atoms as being "typed" by this type system:
+
+    T,U ::=   Fin(n)  | T + U  | T * U  |  T => U
+
+   [[T]]  : Atom.t Set.t
+
+   [[Fin(n)]] = {Base(0), ... , Base(n-1)}
+   [[T + U]]  = {Inl t | t \in [[T]]} \cup {Inr u | u \in [[U]] }
+   [[T * U]]  = {Prod(t,u) | t \in [[T]], u \in [[U]]}
+   [[T => U]] = {Map m | List.map fst (AtomMap.bindings m) = Set.to_list [[T]]}
+
+
+     x < n
+  ---------------
+  Base x : Fin(n)
+  
+       t : T              u : U
+  ---------------    ---------------    
+   Inl t : T + U      Inr u : T + U
+
+
+     t : T    u : U
+  -------------------
+   Prod(t,u) : T * U
+
+
+  domain(m) = [[T]] and forall t in domain(m)   m(t) : U
+  ---------------------------------------------------------
+    Map m : T => U
+
+
+
+ *)
+module
+  rec Atom : sig
+    type t =
+      | Base of int
+      | Inl of t
+      | Inr of t
+      | Prod of t * t
+      | Map of t AtomMap.t
+    
+    val compare : t -> t -> int
+    val to_string : t -> string
+  end =
+  
+  struct
+    type t =
+      | Base of int
+      | Inl of t
+      | Inr of t
+      | Prod of t * t
+      | Map of t AtomMap.t
+    
+    let rec compare t1 t2 =
+      begin match t1, t2 with
+      | Base x, Base y -> Int.compare x y
+      | Base _, _ -> -1
+
+      | Inl _, Base _ -> 1
+      | Inl x, Inl y -> compare x y
+      | Inl _, _ -> -1
+
+      | Inr _, Base _ -> 1
+      | Inr _, Inl _ -> 1
+      | Inr x, Inr y -> compare x y
+      | Inr _, _ -> -1
+
+      | Prod(_,_), Base _ -> 1
+      | Prod(_,_), Inl _ -> 1
+      | Prod(_,_), Inr _ -> 1
+      | Prod(x1,x2), Prod(y1,y2) ->
+         let c1 = compare x1 y1 in
+         if c1 = 0 then compare x2 y2
+         else c1
+      | Prod(_,_), _ -> -1
+
+      | Map x, Map y -> AtomMap.compare compare x y
+      | Map _, _ -> 1
+      end
+
+    let rec to_string t =
+      begin match t with
+      | Base x -> Int.to_string x
+      | Inl x -> "Inl " ^ (to_string x)
+      | Inr x -> "Inr " ^ (to_string x)
+      | Prod(x,y) -> "(" ^ (to_string x) ^ "," ^ (to_string y) ^ ")"
+      | Map m ->
+         let s = String.concat ", "
+                   (List.map 
+                      (fun (k,v) -> (to_string k) ^ "->" ^ (to_string v))
+                      (AtomMap.bindings m) )
+         in
+         "[" ^ s ^ "]"
+      end
+         
+    
+  end
+
+and AtomMap : Map.S with type key = Atom.t = Map.Make(Atom)
+
+module AtomSet : Set.S with type elt = Atom.t = Set.Make(Atom)
+
+
