ml/CCC.ml
@@ -1,0 +1,102 @@
+module type CCC = sig
+
+  (* These are mostly "phantom types" that don't really have much impact *)
+  type base
+  type one
+  type ('a, 'b) prod
+  type zero
+  type ('a, 'b) sum
+  type ('a, 'b) exp
+
+  (* A category consists of a collection of objects and a collection of hom sets *)
+  type 'a obj
+  type ('a, 'b) hom
+
+  (* There is a notion of equality of morphisms *)
+  val eq2 : ('a obj, 'b obj) hom -> ('a obj, 'b obj) hom -> bool
+
+  (* every object has an identity morphsym *)
+  val id : 'a obj -> ('a obj, 'a obj) hom
+
+  (* There is a way of composing morphisms *)
+  val (>>>) : ('a obj, 'b obj) hom -> ('b obj, 'c obj) hom -> ('a obj, 'c obj) hom
+
+  
+  (* We have various ways of "naming" objects in the category *)
+  (* [b] is some unspecified collection of "atomic" base objects *)
+  val b : int -> base obj
+
+  (* These provide ways of constructing objects in the category *)
+  val u : one obj
+  val z : unit -> zero obj
+  val prod : 'a obj -> 'b obj -> ('a, 'b) prod obj
+  val sum  : 'a obj -> 'b obj -> ('a, 'b) sum obj
+  val exp  : 'a obj -> 'b obj -> ('a, 'b) exp obj
+
+  val zero : (zero obj, 'a obj) hom
+
+  val inl  : 'a obj -> ('a obj, ('a obj, 'b obj) sum obj) hom
+  val inr  : 'b obj -> ('b obj, ('a obj, 'b obj) sum obj) hom
+  val case : ('a obj, 'c obj) hom -> ('b obj, 'c obj) hom -> (('a obj, 'b obj) sum obj, 'c obj) hom
+
+  val unit : 'a obj -> ('a obj, one obj) hom
+
+  val fst  : 'a obj -> 'b obj -> (('a obj, 'b obj) prod obj, 'a obj) hom
+  val snd  : 'a obj -> 'b obj -> (('a obj, 'b obj) prod obj, 'b obj) hom
+  val pair : ('c obj, 'a obj) hom -> ('c obj, 'b obj) hom -> ('c obj, ('a obj, 'b obj) prod obj) hom
+
+  val curry : (('a obj, 'b obj) prod obj, 'c obj) hom -> ('a obj, ('b obj, 'c obj) exp obj) hom
+  val apply : 'a obj -> 'b obj -> ((('a obj, 'b obj) exp obj, 'a obj) prod obj, 'b obj) hom
+
+  (* For debugging *)  
+  val string_of_obj : 'a obj -> string
+  val string_of_hom : ('a, 'b) hom -> (string * string) list
+
+end
+
+module OCaml : CCC =
+
+  struct
+
+    type base = int
+    type one = unit
+    type ('a, 'b) prod = 'a * 'b
+    type zero = | 
+    type ('a, 'b) sum =
+      | Inl of 'a
+      | Inr of 'b
+    type ('a, 'b) exp = 'a -> 'b
+
+    type 'a obj = 'a
+    type ('a, 'b) hom = 'a -> 'b
+
+    let b x = x
+    let u = ()
+    let z () = failwith "no zero obj"
+    let prod x y = (x,y)
+    let sum x y = Inl x
+    let exp x y = fun _ -> y
+    
+    let eq2 f g = false
+    let id x = fun a -> a
+
+    let (>>>) f g = fun x -> g (f x)
+    
+    let zero = fun z -> begin match z with | _ -> failwith "ZERO" end
+
+    let inl _  = fun x -> Inl x
+    let inr _ = fun y -> Inr y
+    let case f g = fun a -> begin match a with | Inl x -> f x | Inr y -> g y end
+
+    let unit _ = fun _ -> ()
+
+    let fst _ _ (x, y) = x
+    let snd _ _ (x, y) = y
+    let pair f g = fun c -> (f c, g c)
+
+    let curry f = fun x y -> f (x, y)
+    let apply _ _ (f, x) = f x
+
+    let string_of_obj _ = "<obj>"
+    let string_of_hom _ = [("in", "ou")]
+  end
