ml/Denotation.ml
@@ -1,0 +1,18 @@
+;; open STLC
+;; open CCC
+
+
+module Denote (C : CCC) = struct
+
+  let rec denote_typ (t:typ) : C.obj =
+    begin match t with
+    | Base n -> C.b n
+    | Zero   -> C.z ()  (* Thunked? *)
+    | Plus(t, u) -> C.sum (denote_typ t) (denote_typ u)
+    | One -> C.u
+    | Prod(t, u) -> C.prod (denote_typ t) (denote_typ u)
+    | Arr(t, u) -> C.exp (denote_typ t) (denote_typ u)
+    end
+
+
+end  
