ml/FinSet.ml
@@ -1,0 +1,151 @@
+;; open Atom
+;; open CCC
+
+module FinSet : CCC = struct
+
+  type base = Atom.t
+  type one = Atom.t
+  type ('a, 'b) prod = Atom.t
+  type zero = Atom.t
+  type ('a, 'b) sum = Atom.t
+  type ('a, 'b) exp = Atom.t
+
+  type 'a obj = AtomSet.t
+  type ('a, 'b) hom = Atom.t AtomMap.t
+
+  let eq2 f g = AtomMap.compare Atom.compare f g = 0
+
+  let id a = AtomSet.fold (fun x m -> AtomMap.add x x m)  a AtomMap.empty
+  let (>>>) f g =
+    AtomMap.fold (fun k v m ->
+        AtomMap.add k (AtomMap.find v g) m) f AtomMap.empty
+
+  (* In FinSet, [b x] is the Finite Set {0, 1, ..., x} *)
+  let b x =
+    let rec loop n acc =
+      if n = 0 then acc else loop (n-1) (AtomSet.add (Atom.Base (n-1)) acc)
+    in
+    loop x AtomSet.empty
+
+  (* one is the same as the singleton set {0} *)
+  let u = b 1
+  
+  let zero = AtomMap.empty
+
+  (* the disjoint union of two sets *)
+  let sum a b =
+    AtomSet.union
+      (AtomSet.map (fun x -> Atom.Inl x) a)
+      (AtomSet.map (fun y -> Atom.Inr y) b)
+
+  let inl a = AtomSet.fold (fun x m -> AtomMap.add x (Atom.Inl x) m) a AtomMap.empty
+  let inr b = AtomSet.fold (fun x m -> AtomMap.add x (Atom.Inr x) m) b AtomMap.empty
+  let case f g =
+    let m = AtomMap.fold (fun k v m -> AtomMap.add (Atom.Inl k) v m) f AtomMap.empty in
+    AtomMap.fold (fun k v m -> AtomMap.add (Atom.Inr k) v m) g m
+
+  
+  let unit a = AtomSet.fold (fun x m -> AtomMap.add x (Atom.Base 0) m) a AtomMap.empty
+
+  (* the cartesian product of two finite sets *)
+  let prod (a : 'a obj) (b  : 'b obj) : ('a, 'b) prod obj =
+    AtomSet.fold
+      (fun ai s ->
+        AtomSet.fold
+          (fun bj s ->
+            AtomSet.add (Atom.Prod(ai, bj)) s)
+          b s)
+      a AtomSet.empty
+  
+  let fst a b =
+    AtomSet.fold (fun x m ->
+        AtomSet.fold (fun y m -> AtomMap.add (Atom.Prod(x,y)) x m) b m) a AtomMap.empty
+
+  let snd a b =
+    AtomSet.fold (fun x m ->
+        AtomSet.fold (fun y m -> AtomMap.add (Atom.Prod(x,y)) y m) b m) a AtomMap.empty
+  
+  (* Assumes that dom(f) and dom(g) are the same! *)
+  let pair f g =
+    AtomMap.fold (fun k x m -> AtomMap.add x (Atom.Prod(x, AtomMap.find k g)) m) f AtomMap.empty
+
+
+
+  (* The exponential object in finite sets [a -> b] is the set of all maps from [a] to [b].
+     It has cardinality [a -> b] = (cardinality b) ^ (cardinality a) 
+  *)
+  (* 
+     Given sets [a] and [b] computes the set of all functions [a -> b] represented 
+     as Atom.Map m where m is a Atom.t AtomMap.t.
+
+     If [a] is {a1, ... , an} and [b] is {b1, ... , bm} then we 
+
+     build the set of all functions [a] to [b] by recursively building the set of all
+     functions F from {a2, ..., an} to [b] and then for each such f we add
+       f + a1 -> b1
+       f + a1 -> b2
+       f + a1 -> ...
+       f + a1 -> bn
+     to the set
+
+  *)
+  let exp (a : 'a obj) (b : 'b obj) :  AtomSet.t =
+    let base = AtomSet.singleton (Atom.Map (AtomMap.empty)) in
+    let extend (ai : Atom.t) (f : Atom.t AtomMap.t) : AtomSet.t =
+      AtomSet.fold (fun bj s -> AtomSet.add (Atom.Map (AtomMap.add ai bj f)) s) b AtomSet.empty
+    in
+    let accumulate (ai : Atom.t) (fs : AtomSet.t) : AtomSet.t =
+      AtomSet.fold (fun f s ->
+          begin match f with
+          | Atom.Map fm ->  AtomSet.union (extend ai fm) s
+          | _ -> failwith "accumulate found non-map"
+          end
+        ) fs AtomSet.empty
+    in
+    AtomSet.fold accumulate a base
+
+  (* f is an Atom.t AtomMap.t where the domain is assumed to be a cartesian product
+     of [a * b] and the range is [c].  It produces a new map with doman [a] and 
+     range [b -> c] by "reassociating the map" and collecting the resulting map
+     [b -> c].
+   *)
+  let curry f  =
+    AtomMap.fold (fun k z m ->
+        begin match k with
+        | Atom.Prod(x, y) ->
+           AtomMap.update x 
+             (fun opt ->
+               begin match opt with
+               | None                 -> Some (Atom.Map(AtomMap.singleton y z))
+               | Some (Atom.Map(exp)) -> Some (Atom.Map(AtomMap.add y z exp))
+               | _ -> failwith "curry: not a map!"
+               end)
+             m
+        | _ -> failwith "curry: input not a product!"
+        end) f AtomMap.empty
+
+  (* The "apply" morphism in finite sets is basically a big lookup table, where the
+     keys are pairs of the form (f, a) where f is a map [a -> b] and each such pair
+     is sent by the map to (f a).  The size of the apply map is thus 
+
+   *)  
+  let apply a b =
+    let exp = exp a b in
+    let pairs = prod exp a in
+    let app p =
+      begin match p with
+      | Atom.Prod(Atom.Map m, a) -> AtomMap.find a m
+      | _ -> failwith "app: ill-formed pair"
+      end
+    in
+    AtomSet.fold (fun p m -> AtomMap.add p (app p) m) pairs AtomMap.empty
+
+  let string_of_obj o =
+    let s = String.concat ", " (List.map Atom.to_string (AtomSet.elements o)) in
+    "{" ^ s ^ "}"
+
+  let string_of_hom (m : Atom.t AtomMap.t) : (string * string) list =
+    let ls = AtomMap.bindings m in
+    List.map (fun (k,v) -> (Atom.to_string k, Atom.to_string v)) ls
+  
+end
