ml/STLC.ml
@@ -1,0 +1,66 @@
+
+(* Types *)
+type typ =
+  | Base of int
+  | Zero
+  | Plus of typ * typ
+  | One
+  | Prod of typ * typ
+  | Arr  of typ * typ
+
+
+type ctx = typ list
+
+(* Terms - these are translated from a dependently typed syntax *)
+type var =
+  | Z
+  | S of var
+
+type lit = int * typ
+
+type tm =
+  | Const of lit    (* Const(i,t) : t *)
+  | Var of var
+  | Err of tm       (* Abort *)
+  | Inl of typ * typ * tm
+  | Inr of typ * typ * tm
+  (* case t1 t2 t (e : (t1+t2)) (br1 : t1 |- t) (br2 : t2 |- t) *)  
+  | Case of typ * typ * typ * tm * tm * tm
+  | Unit
+  | Fst of typ * typ * tm
+  | Snd of typ * typ * tm
+  | Pair of typ * typ * tm * tm
+  | Abs of tm * tm * tm
+  | App of typ * typ * tm * tm
+
+
+(*
+  (* var g2 t -> var (g1 ++ g2) t *)
+  let rec weaken_var_l (g1 : ctx) (* g2 : ctx *) (v:var) : var =
+    begin match g1 with
+    | [] -> v
+    | _::g1' -> S (weaken_var_l g1' v)
+    end
+
+  (* var g1 t -> var (g1 ++ g2) t *)
+  let rec weaken_var_r (* (g1 g2 : ctx) *) (v:var) : var = v
+
+  (* var [u1]++[u2]++g t -> var [u2]++[u1]++g t *)
+  let swap_var (* (g:ctx) *) (v:var) : var =
+    begin match v with
+    | Z -> S Z
+    | S Z -> Z
+    | S n -> v
+    end
+
+  (*
+      var ([u1] ++ G1 ++ [u2] ++ G2) t ->
+      var ([u2] ++ G1 ++ [u1] ++ G2) t.                                           
+                               *)
+  let rec exchange_var_r (g:ctx) (v:var) : var =
+    begin match g with
+    | [] -> swap_var v
+    | _::g1' -> 
+
+ *)
+
