ml/StringLib.ml
@@ -1,0 +1,12 @@
+
+
+(* This isn't very efficient *)
+let string_sep_of_list (p : 'a -> string) (sep : string) (l : 'a list) =
+  let rec loop l acc = 
+    begin match l with
+    | [] -> acc
+    | x::[] -> acc ^ (p x)
+    | x::tl -> loop tl (acc ^ (p x) ^ sep)
+    end
+  in
+  loop l ""
