ml/Unification.ml
@@ -1,0 +1,298 @@
+type var = int
+
+type tm =
+  | Var of var
+  | Leaf of int
+  | Pair of tm * tm
+
+(* Invariants: 
+    - the substitution is sorted by vars 
+    - if (x, Var y) is in the list, then x <> y
+*)
+type subst = (var * tm) list
+
+let empty : subst = []
+
+let check (x:var) (t:tm) : bool =
+  t = Var x
+
+let rec contains (t:tm) (x:var) : bool =
+  begin match t with
+  | Var y -> x = y
+  | Leaf _ -> false
+  | Pair(t1, t2) -> (contains t1 x) || (contains t2 x)
+  end
+
+let assign (s:subst) (x:var) (t:tm) : subst =
+
+  let rec assign' (s:subst) =
+    begin match s with
+    | [] -> [(x, t)]
+    | (y,u)::rest ->
+       if x = y then (y,t)::rest else
+       if x < y then (x,t)::(y,u)::rest
+       else (y,u)::(assign' rest)
+    end
+  in
+  if check x t then failwith "illegal identity assignment" else 
+    assign' s
+
+let rec lookup (s : subst) (x:var) : tm =
+  begin match s with
+  | [] -> Var x
+  | (y,u)::rest ->
+     if x = y then u else
+     if x < y then Var x
+     else lookup rest x
+  end
+
+let rec apply (s : subst) (t:tm) : tm =
+  begin match t with
+  | Var x -> lookup s x
+  | Leaf _ -> t
+  | Pair(t1, t2) -> Pair(apply s t1, apply s t2)
+  end
+
+let rec compose_subst (s1:subst) (s2:subst) : subst =
+  begin match s1 with
+  | [] -> s2
+  | (x,t)::s1' ->
+     begin match s2 with
+     | [] -> s1
+     | (y,u)::s2' ->
+        if x = y then failwith "non-disjoint substitution composition!" else
+          if x < y then (x, apply s2 t)::compose_subst s1' s2 else
+            (y,u)::(compose_subst s1 s2')
+     end
+  end
+
+let bind (m:'a option) (k: 'a -> 'b option) : 'b option =
+  begin match m with
+  | None -> None
+  | Some x -> k x
+  end
+
+let elim (x:var) (t:tm) : (tm * tm) list -> (tm * tm) list  =
+  List.map (fun (t1,t2) -> (apply [(x,t)] t1, apply [(x,t)] t2))
+
+let elim_s (x:var) (t:tm) : subst -> subst =
+  List.map (fun (y,u) -> (y, apply [(x,t)] u))
+
+
+let rec unify (eqns:(tm * tm) list) (so:subst option) : subst option =
+  begin match so with
+  | None -> None
+  | Some s ->
+     begin match eqns with
+       | [] -> Some s
+       | (t1,t2)::eqns' ->
+          begin match t1 with
+          | Var x ->
+             if t2 = Var x then unify eqns' so else
+             if contains t2 x then None else   (* occurs check *)
+             unify (elim x t2 eqns') (Some (assign (elim_s x t2 s) x t2))             
+          | Leaf n ->
+             begin match t2 with
+             | Var y -> unify ((t2, t1)::eqns') so
+             | Leaf m ->
+                if n = m then unify eqns' so else None
+             | Pair(_,_) -> None
+             end
+          | Pair(t11, t12) ->
+             begin match t2 with
+             | Var y ->  unify ((t2, t1)::eqns') so
+             | Leaf _ -> None
+             | Pair(t21, t22) ->
+                unify ((t11, t21)::(t12, t22)::eqns') so
+             end
+          end
+     end
+  end
+
+
+type tm_ =
+  | Conflict_ of tm * tm
+  | Var_ of var
+  | Leaf_ of int
+  | Pair_ of tm_ * tm_
+
+let rec inc (t:tm) : tm_ =
+  begin match t with
+  | Var x -> Var_ x
+  | Leaf n -> Leaf_ n
+  | Pair (t11, t12) -> Pair_ (inc t11, inc t12)
+  end
+
+let rec apply_ (s:subst) (u : tm_) : tm_ =
+  begin match u with
+  | Conflict_ (t1, t2) -> Conflict_ (apply s t1, apply s t2)
+  | Var_ y -> inc (lookup s y)
+  | Leaf_ n -> u
+  | Pair_ (u11, u12) -> Pair_ (apply_ s u11, apply_ s u12)
+  end
+
+let rec i_unify (t1:tm) (t2:tm) (k : tm_ * subst -> 'a) : 'a =
+  begin match t1 with
+  | Var x ->
+     begin match t2 with
+     | Var y ->
+        if x = y then k (Var_ x, [])
+        else if x < y then k (Var_ x, [(y, Var x)])
+        else k (Var_ y, [(x, Var y)])
+
+     | t2' ->
+        if contains t2 x
+        then k (Conflict_ (t1 ,t2), [])   (* This is the case where there is a cycle *)
+        else k (inc t2', [(x, t2')])
+     end
+
+  | Leaf n ->
+     begin match t2 with
+     | Var y ->
+        k (Leaf_ n, [(y, Leaf n)])
+        
+     | Leaf m ->
+        if n = m
+        then k (Leaf_ n, [])
+        else k (Conflict_ (t1, t2), [])
+
+     | Pair(_,_) ->
+        k (Conflict_(Leaf n, t2), [])
+     end
+     
+  | Pair(t11, t12) ->
+     begin match t2 with
+     | Var y ->
+        if contains t1 y
+        then k (Conflict_ (t1, t2), [])
+        else k (inc t2, [(y, t2)])
+        
+     | Leaf _ ->
+        k (Conflict_(t1, t2), [])
+        
+     | Pair(t21, t22) ->
+        i_unify t11 t21
+          (fun (lft, s1) ->
+            i_unify (apply s1 t12) (apply s1 t22)
+              (fun (rgt, s2) ->
+                k (Pair_(apply_ s2 lft, rgt), compose_subst s1 s2)))
+     end     
+  end
+
+
+(*
+  (x, x) = ((1, 2), 3)
+  ==>
+  ((1,2),CC[(1,2)|3]) , [x=(1,2)]
+  -of-
+  (3, CC[3 | (1,2)])  , [x=3]
+
+
+  (x, (y, y)) = ((y, y), (1, 2))
+  ==>
+  
+
+
+
+  (x, (x,x)) = (1, (2, 3))
+   ==>
+  (x, (-,-)), [x=1], [(rl->(1,2)), (rr->(1,3))
+
+ -or-
+  (-, (x,-)), [x=2], [(l->(1,2)), (rr->(2,3))]
+
+ -or-
+  (-, (-, x)), [x=3], [(l->(1,3)), (rl->(2,3))]
+
+
+  (x, (x,x)) = ((1,2), (2, (1,3)))
+   ==>
+  (x, (-,-)), [x = (1,2)], [rl->((1,2),2), rrr->(2,3)]
+  -or-
+  (-, (x,-)), [x = 2], [l->(2,(1,2)), rr->(2,(1,3))]
+  -or-
+  (-, (-,x)), [x = (1,3)], [lr->(3,2), rl->((1,3),2)]
+
+ 
+
+
+
+  ((x, (x, x)), (y, 1)) = ((1, (2, 3), (x, x)))
+  ==>
+  ((x, (-, -)), (y, 1)), [x->1, y->1], [lrl->(1,2), lrr->(1,3)]
+  -or-
+  ((1, (-, -)), (y, x)), [x->1, y->1], [lrl->(1,2), lrr->(1,3)]
+  -or-
+  ((-, (x, -)), (y, -)), [x->2, y->2], [ll->(1,2), lrr->(2,3), rr->(1,2)]
+  -or-
+  ((-, (-, x)), (y, -)), [x->3, y->3], [ll->(1,3), lrl->(2,3), rr->(1,3)]
+  -or-
+  
+
+  (x,x) = (y,1)
+     [x->1, y->1]
+
+
+  (x, (x,x)) , [(x, [1;2;3]))
+
+  (x, (y,z)) = (1, (2, 3))
+   ==>
+  (x, (y, z)), [(x, [1]); (y, [2]); (z, [3])]
+
+  (1, (2, 3)) = (3, 2, 1))
+   ==>
+  (a, (2, b)), [(a,[(1,3)]); (b,[(3,1)]]]
+
+ *)
+
+
+(*
+
+let rec unify (t1:tm) (t2:tm) : subst option =
+  begin match t1 with
+  | Var x ->
+     begin match t2 with
+     | Var y -> if x = y then Some [] else Some (assign empty x t2)
+     | Leaf -> Some (assign empty x t2)
+     | Pair(_,_) -> Some (assign empty x t2)
+     end
+  | Leaf ->
+     begin match t2 with
+     | Var y -> Some (assign empty y t1)
+     | Leaf -> Some empty
+     | Pair(_,_) -> None
+     end
+  | Pair(t11, t12) ->
+     begin match t2 with
+     | Var y -> Some (assign empty y t1)
+     | Leaf -> None
+     | Pair(t21, t22) ->
+        bind (unify t11 t21)
+          (fun s ->
+            let t12' = apply s t12 in
+            let t22' = apply s t22 in
+            bind (unify t12' t22')
+           (fun s' -> -> combine s s'))
+     end
+  end
+and combine (s1 : subst) (s2 : subst) : subst option =
+  begin match s1, s2 with
+  | [], [] -> Some []
+  | [], s2 -> Some s2
+  | s1, [] -> Some s1
+  | (x,t)::r1, (y,u)::r2 ->
+     if x < y then bind (combine r1 s2) (fun s -> (x,t)::s) else
+     if x = y then
+ *)     
+
+
+let ex1 : tm = Pair(Var 0, Pair(Var 1, Var 1))
+let ex2 : tm = Pair(Pair(Leaf 0, Leaf 0), Var 0)
+let ex3 : tm = Pair(Pair(Var 0, Var 1), Var 1)     
+let ex4 : tm = Pair(Pair(Var 0, Var 1), Pair(Leaf 0,Var 1))
+let ex5 : tm = Pair(Var 0, Var 0)
+let ex6 : tm = Pair(Var 1, Leaf 0)
+let ex7 : tm = Pair(Var 0, Pair (Var 1, Var 2))
+let ex8 : tm = Pair(Var 1, Pair (Var 2, Var 0))
+let ex9 : tm = Pair(Leaf 1, Pair (Leaf 2, Leaf 3))
+
