coq/Relations.v
@@ -1,0 +1,216 @@
+From Coq Require Import
+     Relations.Relation_Definitions
+     Classes.RelationClasses.
+
+Definition lub {A : Type} (lt : relation A) (a b c : A) : Prop :=
+  lt a c /\ lt b c /\ (forall d, lt a d -> lt b d -> lt c d).
+
+Definition LT {A : Type} (lt : relation A) (X : A -> Prop) (a : A) :=
+  forall x, X x -> lt x a.
+
+Definition LUB {A : Type} (lt : relation A) (X : A -> Prop) (c : A) :=
+  LT lt X c /\ (forall d, LT lt X d -> lt c d).
+
+Definition chain {A : Type} (lt : relation A) := {f : nat -> A | forall i, lt (f i) (f (S i))}.
+Definition elts {A : Type} {lt : relation A} (c : chain lt) (a : A) : Prop :=
+  exists i, proj1_sig c i = a.
+
+Definition complete {A : Type} (lt : relation A) : Prop :=
+  forall (c:chain lt), exists (a:A), LUB lt (elts c) a.
+
+Section CPO.
+  Context {A : Type}.
+  Class CPO (lt : relation A) :=
+    {
+    po :> PreOrder lt;
+    cmp : complete lt;
+    }.
+End CPO.
+
+Instance CPO_nat : CPO (fun (x y:nat) => x = y).
+constructor.
+constructor.
+constructor.
+repeat intro. subst; reflexivity.
+intro. destruct c. exists (x 0).
+repeat red. unfold LT, elts. split; intros.
+- destruct H. cbn in H. subst. induction x1. reflexivity.
+  rewrite <- e. assumption.
+- apply H. exists 0. cbn. reflexivity.
+Qed.
+
+Section PreOrderEQ.
+  Context {A : Type}.
+  Context {lt : relation A}.
+  Context {PR : PreOrder lt}.
+
+  Definition pre_eq : relation A :=
+    fun a b => lt a b /\ lt b a.
+
+  Global Instance pre_eq_refl : Reflexive(pre_eq).
+  Proof.
+    destruct PR.
+    constructor; reflexivity.
+  Qed.
+
+  Global Instance pre_eq_trans : Transitive(pre_eq).
+  Proof.
+    destruct PR.
+    constructor; destruct H, H0; eapply transitivity; eauto.
+  Qed.
+
+  Global Instance pre_eq_symm : Symmetric(pre_eq).
+  Proof.
+    destruct PR.
+    constructor; destruct H; tauto.
+  Qed.
+End PreOrderEQ.
+  
+    
+          
+
+Section Continuous.
+
+  
+
+
+  
+
+  
+
+
+  
+  
+  
+  
+
+
+
+Definition set (A:Type) := A -> Prop.
+
+Definition dual {A : Type} (v : set A) : set A -> Prop :=
+  fun (f : A -> Prop) => forall (a:A), v a <-> f a.
+
+Definition join {A : Type} (X : set A -> Prop) : set A :=
+  fun (a:A) => exists (g : A -> Prop), X g /\ g a.
+
+Definition meet {A : Type} (X : set A -> Prop) : set A :=
+  fun (a:A) => forall (g : A -> Prop), X g -> g a.
+
+Definition meet_closed {A : Type} (v : set A) :=
+  forall (a:A), v a <-> (meet (dual v) a).
+
+Lemma all_meet_closed : forall A (v : set A), meet_closed v.
+Proof.
+  unfold meet_closed, meet, dual.
+  intros.
+  split; intros.
+  - apply H0. assumption.
+  - specialize (H v). apply H. tauto.
+Qed.
+
+
+Definition join_closed {A : Type} (v : set A) :=
+  forall (a:A), v a <-> (join (dual v) a).
+
+Lemma all_join_closed : forall A (v : set A), join_closed v.
+Proof.
+  unfold join_closed, join, dual.
+  intros.
+  split; intros.
+  - exists v. split; tauto.
+  - repeat destruct H. apply H. assumption.
+Qed.    
+
+Definition HRelation (A B : Type) := A -> B -> Prop.
+
+Definition T' {A B : Type} (R : HRelation A B) : HRelation (A -> Prop) (B -> Prop) :=
+  fun f g =>
+    (forall a, f a -> exists b, R a b /\ g b) /\ (forall b, g b -> exists a, R a b /\ f a).
+
+Definition T {A B : Type} (R : HRelation A B) : HRelation (A -> Prop) (B -> Prop) :=
+  fun f g => forall a b, R a b <-> (f a) <-> (g b).
+
+
+
+Definition TT {A B : Type} (R : HRelation A B) : HRelation A B :=
+  fun a b => forall f g, (T R f g) -> (f a) <-> (g b).
+
+Lemma R_TT: forall {A B : Type} (R : HRelation A B) a b (H : R a b), (TT R a b).
+Proof.
+  intros A B R.
+  unfold TT, T.
+  intros.
+  split; intros.
+    + eapply H0. split; intros. apply H1. auto.
+    + apply H0 in H. assumption. assumption.
+Qed.      
+  
+Definition TT_closed {A B : Type} (R : HRelation A B) :=
+  forall a b, (TT R a b) -> R a b.
+
+Definition rel {A B : Type} (f : A -> B) : HRelation A B :=
+  fun a b => (f a) = b.
+
+Lemma TT_closed_rel : forall A B (R : HRelation A B), TT_closed R.
+Proof.
+  intros A B R.
+  unfold TT_closed, TT, T.
+  intros.
+  split; intros.
+  - split; intros.
+    + eapply H0. split; intros. apply H1. auto.
+    + apply H0 in H. assumption. assumption.
+  - specialize (H (fun x => R x b) (fun y => y = b)). cbn in *.
+    apply H. intros. split. intros.
+
+
+Lemma TT_closed_rel : forall A B (f : A -> B), TT_closed (rel f).
+Proof.
+  intros A B f.
+  unfold TT_closed, TT, T, rel.
+  intros.
+  split; intros.
+  - split; intros.
+    + eapply H0. split; intros. apply H1. auto.
+    + apply H0 in H. assumption. assumption.
+  - 
+
+Definition TT' {A B : Type} (R : HRelation A B) : HRelation A B :=
+  fun a b => forall f g, (T' R f g) -> (f a) <-> (g b).
+
+Definition TT'' {A B : Type} (R : HRelation A B) : HRelation A B :=
+  fun a b => 
+
+
+
+Definition TT'_closed {A B : Type} (R : HRelation A B) :=
+  forall a b, R a b <-> (TT' R a b).
+
+
+Lemma TT'_closed_rel : forall A B (f : A -> B), TT'_closed (rel f).
+Proof.
+  intros A B f.
+  unfold TT'_closed, TT', T', rel.
+  intros.
+  split; intros.
+  - split; intros.
+    + subst. destruct H0. apply H in H1. destruct H1 as [b [Ha Hb]]. subst. assumption.
+    + subst. destruct H0. apply H0 in H1. destruct H1 as [b [Ha Hb]]. subst. 
+
+
+Lemma TT_closed_rel : forall A B (f : A -> B), TT_closed (rel f).
+Proof.
+  intros A B f.
+  unfold TT_closed, TT, T, rel.
+  intros.
+  split; intros.
+  - split; intros.
+    + subst. eapply H0. reflexivity. assumption.
+    + subst. eapply H0. reflexivity. assumption.
+  - specialize (H (fun a' => True) (fun b' => b = b' -> f a = b)). 
+    cbn in H.
+    apply H; auto.
+    intros. split; auto. intros. subst. 
+    intros. subst. reflexivity.
+                                            
